lib.v
@@ -15,3 +15,18 @@ Tactic Notation "solve" "by" "inversion" "3" :=
   solve_by_inversion_step (solve by inversion 2).
 Tactic Notation "solve" "by" "inversion" :=
   solve by inversion 1.
+
+
+(* to simplify the handling of _quote / _typecheck = Some _ *)
+Ltac option_match H n :=
+  let OE := fresh "o" n in
+  let E := fresh n in
+  match type of H with
+    (match ?oe with
+     | Some _ => _
+     | None => None
+     end = _ ) =>
+    remember oe as OE;
+    destruct OE as [E |];
+    inversion H
+  end.
