unquote.v
@@ -213,11 +213,118 @@ Proof.
 Qed.
 
 
+Lemma unquoted_wrapper : forall t e e',
+    exp_subst e injection_symbol identity e' ->
+    (exp_app (exp_tapp unquote t)
+             (exp_func injection_symbol identity_type e)) ~ e'.
+Proof.
+  intros t e e' H0.
+  remember (exp_func "q" (type_func identity_type t)
+                     (exp_app (exp_var "q") identity)) as m.
+  assert ((exp_tapp unquote t) ~ m).
+  {
+    apply equiv_base.
+    apply bn_base.
+    constructor.
+    rewrite Heqm.
+    apply tse_func.
+    auto.
+    unfold identity.
+    unfold identity_type_var.
+    unfold identity_type_symbol.
+    eapply tse_app.
+    auto.
+    eapply tse_tfunc_p.
+    congruence.
+    auto.
+  }
+  subst.
+  rewrite H.
+  econstructor 3.
+  repeat econstructor; try (intros contra; inversion contra).
+  fold identity.
+  repeat constructor.
+  auto.
+Qed.
+
+
+Lemma identity_reduce : forall e t,
+    (exp_app (exp_tapp identity t) e) ~ e.
+Proof.
+  intros e t.
+  constructor.
+  econstructor 2; repeat constructor.
+Qed.
+
+
+Lemma unquoted_free_eq : forall t e e' env,
+    no_injection_symbol e ->
+    _typecheck env e = Some t ->
+    _quote env e = Some e' ->
+    (subst_exp e' injection_symbol identity) ~ e.
+Proof.
+  intros t e e' env Hi Ht He.
+  generalize dependent t.
+  generalize dependent e'.
+  generalize dependent env.
+  induction e; intros env e' He t0 Ht;
+    inversion Hi; subst; simpl in *.
+  + unfold option_map in He.
+    remember ({a, t | env}) as env'.
+    option_match He e.
+    option_match Ht t.
+    subst.
+    simpl.
+    destruct (ascii_dec a injection_symbol); try contradiction.
+    symmetry in Heqoe, Heqot.
+    rewrite (IHe H3 _ _ Heqoe _ Heqot).
+    reflexivity.
+  + option_match He t1.
+    option_match He e1.
+    option_match He e2.
+    destruct t1 as [|t10 t11|]; inversion Ht; subst.
+    option_match Ht t2.
+    clear He H0 H3.
+    simpl.
+    symmetry in Heqoe1, Heqoe2, Heqot1, Heqot2.
+    rewrite (IHe1 H1 _ _ Heqoe1 _ Heqot1).
+    rewrite (IHe2 H2 _ _ Heqoe2 _ Heqot2).
+    rewrite identity_reduce.
+    reflexivity.
+  + unfold option_map in He.
+    option_match Ht t.
+    option_match He e.
+    simpl.
+    symmetry in Heqoe, Heqot.
+    rewrite (IHe H0 _ _ Heqoe _ Heqot).
+    reflexivity.
+  + option_match He t.
+    option_match He e.
+    destruct t1; inversion Ht.
+    simpl.
+    rewrite identity_reduce.
+    symmetry in Heqoe, Heqot.
+    rewrite (IHe H0 _ _ Heqoe _ Heqot).
+    reflexivity.
+  + inversion He.
+    simpl.
+    destruct (ascii_dec a injection_symbol); try contradiction.
+    reflexivity.
+Qed.
+
+      
 Theorem unquoted_eq : forall e e' t,
+    no_injection_symbol e ->
     quote e = Some e' ->
     typecheck e = Some t ->
     (exp_app (exp_tapp unquote t) e') ~ e.
-Admitted.
-
-      
+Proof.
+  intros e e0' t0 Hi Hq Ht.
+  unfold quote in Hq.
+  unfold option_map in Hq.
+  option_match Hq e'.
+  constructor 3 with (subst_exp e' injection_symbol identity).
+  apply unquoted_wrapper; try (apply subst_exp_correct; auto).
+  eapply unquoted_free_eq; eauto.
+Qed.
 
